website/code/Logic-in-Dafny.dfy
@@ -1,0 +1,34 @@
+datatype Peano = 
+  | Zero
+  | Succ (Peano)
+
+/** Quiz:
+
+a.  Is Succ(Zero) equal to Succ(Zero)?
+
+b.  Is Succ(Zero) equal to Zero?
+
+c.  Does there exist a Peano number n such that Succ(n) is equal to Zero?
+
+d.  If Succ(zero) is equal to Succ(x), do we know something about x?
+
+e.  Let's define another datatype: 
+    
+    datatype Positive = 
+    | One 
+    | Inc(Positive)
+
+    Is One an element of the Peano datatype?
+
+f.  How do you prove things about Peano?
+ */
+
+function SumUpTo(counter: int, upTo: int): int
+    //What decreases clause is needed here?
+  {
+    if upTo <= counter then
+      counter
+    else
+      counter + SumUpTo(counter + 1, upTo)
+  }
+
